Delta correctness progress -- equivalence of schemes (regular <--> Rq)

Security/SaberRqDeltaCorrectness.ec
@@ -3,13 +3,17 @@
 (* ----------------------------------- *)
 
 (* --- Built-in --- *)
-require import AllCore Distr ZModP IntDiv StdOrder.
+require import AllCore Distr ZModP IntDiv StdOrder List.
 
 (* --- Local --- *)
 require import SaberRqPreliminaries.
+(*---*) import Saber_PKE.
 (*---*) import Mat_Rp Mat_Rq.
-(*---*) import Rp Rq.
-(*---*) import Zp Zq.
+(*---*) import Zp Rp Rp.ComRing Rp.BasePoly.
+(*---*) import Zq Rq Rq.ComRing Rq.BasePoly. 
+(*---*) import Zppq Rppq Rppq.ComRing Rppq.BasePoly.
+(*---*) import Z2t R2t R2t.ComRing R2t.BasePoly.
+(*---*) import Z2 R2 R2.ComRing R2.BasePoly.
 
 (* ----------------------------------- *)
 (*  Adversary Prototypes               *)
@@ -47,3 +51,210 @@ module Saber_PKE_Correctness (A : Adv_Cor) = {
 lemma shl_shr_error (x : int, ex : int) : shl (shr x ex) ex = x - (x %% 2 ^ ex).
 proof. by rewrite /shr /shl divzE. qed.
 
+(* ----------------------------------- *)
+(* All Rq                              *)
+(* ----------------------------------- *)
+
+pragma Goals:printall.
+
+op scaleZq2Z2 (z : Zq) : Z2 = Z2.inzmod (scale (Zq.asint z) eq 1).
+op scaleZq2Z2t (z : Zq) : Z2t = Z2t.inzmod (scale (Zq.asint z) eq (et + 1)).
+
+op scaleRq2R2 (p : Rq) : R2 =
+  BigR2.XnD1CA.bigi predT (fun i => scaleZq2Z2 p.[i] ** exp R2.iX i) 0 n. 
+op scaleRq2R2t (p : Rq) : R2t =
+  BigR2t.XnD1CA.bigi predT (fun i => scaleZq2Z2t p.[i] ** exp R2t.iX i) 0 n. 
+
+op scale_up (x : int, ea : int, eb : int) : int = shl x (ea - eb).
+
+op scaleZ22Zq (z : Z2) : Zq = Zq.inzmod (scale_up (Z2.asint z) eq 1).
+op scaleZ2t2Zq (z : Z2t) : Zq = Zq.inzmod (scale_up (Z2t.asint z) eq (et + 1)).
+op scaleZp2Zq (z : Zp) : Zq = Zq.inzmod (scale_up (Zp.asint z) eq ep).
+
+op scaleR22Rq (p : R2) : Rq =
+  BigRq.XnD1CA.bigi predT (fun i => scaleZ22Zq p.[i] ** exp Rq.iX i) 0 n.
+op scaleR2t2Rq (p : R2t) : Rq =
+  BigRq.XnD1CA.bigi predT (fun i => scaleZ2t2Zq p.[i] ** exp Rq.iX i) 0 n.
+op scaleRp2Rq (p : Rp) : Rq =
+  BigRq.XnD1CA.bigi predT (fun i => scaleZp2Zq p.[i] ** exp Rq.iX i) 0 n.
+
+op scaleRpv2Rqv (pv : Rp_vec) : Rq_vec = offunv (fun i => scaleRp2Rq pv.[i]).
+
+op scaleZq (z : Zq, ez : int) : Zq = Zq.inzmod (scale_up (Zq.asint z) ez 0).
+ 
+op scaleRq (p : Rq, er : int) : Rq = 
+  BigRq.XnD1CA.bigi predT (fun i => (scaleZq p.[i] er) ** exp Rq.iX i) 0 n.
+
+lemma scale_up_DM (ea eb : int) : morphism_2 (fun x => scale_up x ea eb) Int.(+) Int.(+).
+proof. by move => x y; rewrite /scale_up /shl mulrDl. qed.
+
+lemma scale_DM (x y ea eb : int) : 
+  2 ^ (ea - eb) %| x \/  2 ^ (ea - eb) %| y => scale (x + y) ea eb = scale x ea eb + scale y ea eb.
+proof. by case; rewrite /scale /shr; [apply divzDl | apply divzDr]. qed.
+
+lemma scaleZp2Z2t_DM (z1 z2 : Zp) : 
+  2 ^ (ep - (et + 1)) %| Zp.asint z1 \/  2 ^ (ep - (et + 1)) %| Zp.asint z2 => 
+  scaleZp2Z2t (z1 + z2) = scaleZp2Z2t z1 + scaleZp2Z2t z2.
+proof. 
+case => [divz1 | divz2]; rewrite /scaleZp2Z2t -inzmodD -scale_DM ?(divz1, divz2) //;
+    rewrite addE /p /scale /shr /inzmod /t -exprS 1:ge0_et modz_pow2_div;
+    1, 2, 4, 5: smt(Zp.ge0_asint geet2_ep ge0_et); congr; rewrite modz_dvd_pow; smt(ge0_et).
+qed.
+
+lemma scaleZq2Z2t_DM (z1 z2 : Zq) : 
+  2 ^ (eq - (et + 1)) %| Zq.asint z1 \/  2 ^ (eq - (et + 1)) %| Zq.asint z2 => 
+  scaleZq2Z2t (z1 + z2) = scaleZq2Z2t z1 + scaleZq2Z2t z2.
+proof. 
+case => [divz1 | divz2]; rewrite /scaleZq2Z2t -inzmodD -scale_DM ?(divz1, divz2) //;
+    rewrite addE /q /scale /shr /inzmod /t -exprS 1:ge0_et modz_pow2_div;
+    1, 2, 4, 5: smt(Zq.ge0_asint geet2_ep geep1_eq ge0_et); congr; rewrite modz_dvd_pow; smt(ge0_et).
+qed.
+
+(*
+scaleRp2R2t
+  (dotp (pk_decode pk{2}).`2 (Rqv2Rpv s'L) + Rq2Rp h1 +
+   shl_enc (m_decode m{2}) (ep - 1)) 
+=
+scaleRq2R2t
+  (dotp (scaleRpv2Rqv (pk_decode pk{2}).`2) s'L + scaleRq h1 (eq - ep) +
+   scaleR22Rq (m_decode m{2}))
+*)
+lemma scaleRp2R2t_DM (p1 p2 : Rp) : 
+  ((forall (i : int), 0 <= i < n =>  2 ^ (ep - (et + 1)) %| Zp.asint p1.[i]) \/  
+  (forall (i : int), 0 <= i < n =>  2 ^ (ep - (et + 1)) %| Zp.asint p2.[i])) =>
+  scaleRp2R2t (p1 + p2) = scaleRp2R2t p1 + scaleRp2R2t p2.
+proof.
+case => [divz1 | divz2]; rewrite /scaleRp2R2t eq_sym -BigR2t.XnD1CA.big_split /=;
+    rewrite !BigR2t.XnD1CA.big_seq &(BigR2t.XnD1CA.eq_bigr) /= => i /mem_range rng_i;
+    rewrite -scaleDl eq_sym rcoeffD scaleZp2Z2t_DM ?(divz1, divz2) //.
+qed.
+
+lemma scaleRq2R2t_DM (p1 p2 : Rq) : 
+  ((forall (i : int), 0 <= i < n =>  2 ^ (eq - (et + 1)) %| Zq.asint p1.[i]) \/  
+  (forall (i : int), 0 <= i < n =>  2 ^ (eq - (et + 1)) %| Zq.asint p2.[i])) =>
+  scaleRq2R2t (p1 + p2) = scaleRq2R2t p1 + scaleRq2R2t p2.
+proof.
+case => [divz1 | divz2]; rewrite /scaleRq2R2t eq_sym -BigR2t.XnD1CA.big_split /=;
+    rewrite !BigR2t.XnD1CA.big_seq &(BigR2t.XnD1CA.eq_bigr) /= => i /mem_range rng_i;
+    rewrite -scaleDl eq_sym rcoeffD scaleZq2Z2t_DM ?(divz1, divz2) //.
+qed.
+
+lemma modz_pow2_mul (n p i : int) : 0 <= i => 0 <= p <= n =>
+  ((i %% 2 ^ p) * 2 ^ (n - p)) %% 2 ^ n = (i * 2 ^ (n - p)) %% 2 ^ n.
+proof.
+move => ge0_i rng_p.
+case (p = 0) => [-> /=| neq0_p].
++ by rewrite expr0 /= modzMl.
++ rewrite modzE {1}(_ : 2 ^ n = 2 ^ (n - p) * 2 ^ p) 1:-exprD_nneg; first 3 smt().
+  rewrite {2}mulzC divzMpl. admit.
+  rewrite pdiv_small /=. admit.
+  rewrite modzE mulrBl.
+  rewrite -mulrA -exprD_nneg; first 2 smt().
+  rewrite (addzC p) -addzA /=.
+  rewrite modzE {2}(_ : 2 ^ n = 2 ^ (n - p) * 2 ^ p) 1:-exprD_nneg; first 3 smt().
+  rewrite {3}mulzC divzMpl. admit.
+trivial.
+qed.
+
+lemma scaleZp2Zq_MA (z1 z2 : Zp) : scaleZp2Zq (z1 * z2) = scaleZp2Zq z1 * Zp2Zq z2.
+proof.
+rewrite /scaleZp2Zq /Zp2Zq -inzmodM /scale_up /shl mulrAC mulE -eq_inzmod /p /q  modz_pow2_mul //.
++ smt(Zp.ge0_asint).
++ smt(ge2_ep geep1_eq).
+qed.
+
+
+lemma test1 (v1 : Rp_vec) (v2 : Rq_vec) :
+  scaleRp2Rq (dotp v1 (Rqv2Rpv v2)) = dotp (scaleRpv2Rqv v1) v2.
+proof.
+rewrite /dotp polyXnD1_eqP => i rng_i.
+qed.
+
+
+ 
+module Saber_PKE_Scheme_Rq : Scheme = {
+   proc kg() : pkey * skey = {
+      var sd: seed;
+      var _A: Rq_mat;
+      var s: Rq_vec;
+      var b: Rp_vec;
+      
+      sd <$ dseed;
+      _A <- gen sd;
+      s <$ dsmallRq_vec;
+      b <- scaleRqv2Rpv (_A *^ s + h);
+      
+      return (pk_encode (sd, b), sk_encode s);
+   }
+
+   proc enc(pk: pkey, m: plaintext) : ciphertext = {
+      var pk_dec: seed * Rp_vec;
+      var m_dec: R2;
+
+      var sd: seed;
+      var _A: Rq_mat;
+      var s': Rq_vec;
+      var b, b': Rp_vec;
+      var bq: Rq_vec;
+      var v': Rq;
+      var cm: R2t;
+      
+      m_dec <- m_decode m;
+      pk_dec <- pk_decode pk;
+      sd <- pk_dec.`1;
+      b <- pk_dec.`2;
+      _A <- gen sd;
+      s' <$ dsmallRq_vec;
+      b' <- scaleRqv2Rpv ((trmx _A) *^ s' + h);
+      bq <- scaleRpv2Rqv b;
+      v' <- (dotp bq s') + (scaleRq h1 (eq - ep));
+      cm <- scaleRq2R2t (v' + (scaleR22Rq m_dec));
+      
+      return c_encode (cm, b');
+   }
+
+   proc dec(sk: skey, c: ciphertext) : plaintext option = {
+      var c_dec: R2t * Rp_vec;
+      var cm: R2t;
+      var cmq: Rq;
+      var b': Rp_vec;
+      var bq': Rq_vec;
+      var v: Rq;
+      var s: Rq_vec;
+      var m': R2;
+
+      c_dec <- c_decode c;
+      s <- sk_decode sk;
+      cm <- c_dec.`1;
+      cmq <- scaleR2t2Rq cm;
+      b' <- c_dec.`2;
+      bq' <- scaleRpv2Rqv b';
+      
+      v <- (dotp bq' s) + (scaleRq h1 (eq - ep));
+      m' <- scaleRq2R2 (v  - cmq + (scaleRq h2 (eq - ep)));
+      
+      return Some (m_encode m');
+   }
+}.
+
+
+lemma eq_kg: equiv[Saber_PKE_Scheme.kg ~ Saber_PKE_Scheme_Rq.kg : true ==> ={res}].
+proof.
+by proc; sim.
+qed.
+
+lemma eq_enc: equiv[Saber_PKE_Scheme.enc ~ Saber_PKE_Scheme_Rq.enc : ={pk, m} ==> ={res}].
+proof.
+proc.
+auto; progress. 
+congr; rewrite &(pw_eq) //.
+admit.
+qed.
+
+lemma eq_dec: equiv[Saber_PKE_Scheme.dec ~ Saber_PKE_Scheme_Rq.dec : ={sk, c} ==> ={res}].
+proof.
+proc.
+auto; progress.
+congr.
+admit.
+qed.
